functional-programming-lean/src/SUMMARY.md
@@ -63,5 +63,7 @@
   - [Tail Recursion](programs-proofs/tail-recursion.md)
   - [Proving Equivalence](programs-proofs/tail-recursion-proofs.md)
   - [Arrays and Termination](programs-proofs/arrays-termination.md)
+  - [Safe Array Indices](programs-proofs/fin.md)
+  - [Insertion Sort](programs-proofs/insertion-sort.md)
 
 [Next Steps]()
