functional-programming-lean/src/programs-proofs/insertion-sort.md
@@ -1,0 +1,48 @@
+# Insertion Sort
+
+While insertion sort does not have the optimal worst-case time complexity for a sorting algorithm, it still has a number of useful properties:
+ * It is simple and straightforward to implement and understand
+ * It is an in-place algorithm, requiring no additional space to run
+ * It is a stable sort
+ * It is fast when the input is already almost sorted
+ 
+In-place algorithms are particularly useful in Lean due to the way it manages memory.
+In some cases, operations that would normally copy an array can be optimized into mutation.
+This includes swapping elements in an array.
+
+Most languages and run-time systems with automatic memory management, including JavaScript, the JVM, and .NET, use tracing garbage collection.
+When memory needs to be reclaimed, the system starts at a number of roots (such as the call stack and global values) and then determines which values can be reached by recursively chasing pointers.
+Any values that can't be reached are deallocated, freeing memory.
+
+Reference counting is an alternative to tracing garbage collection that is used by a number of languages, including Python, Swift, and Lean.
+In a system with reference counting, each object in memory has a field that tracks how many references there are it.
+When a new reference is established, the counter is incremented.
+When a reference ceases to exist, the counter is decremented.
+When the counter reaches zero, the object is immediately deallocated.
+
+Reference counting has one major disadvantage compared to a tracing garbage collector: circular references can lead to memory leaks.
+If object \\( A \\) references object \\( B \\) , and object \\( B \\) references object \\( A \\), they will never be deallocated, even if nothing else in the program references either \\( A \\) or \\( B \\).
+Circular references result either from uncontrolled recursion or from mutable references.
+Because Lean supports neither, it is impossible to construct circular references.
+
+Reference counting means that the Lean runtime system's primitives for allocating and deallocating data structures can check whether a reference count is about to fall to zero, and re-use an existing object instead of allocating a new one.
+This is particularly important when working with large arrays.
+
+
+An implementation of insertion sort for Lean arrays should satisfy the following criteria:
+ 1. Lean should accept the function without a `partial` annotation
+ 2. If passed an array to which there are no other references, it should modify the array in-place rather than allocating a new one
+
+The first criterion is easy to check: if Lean accepts the definition, then it is satisfied.
+The second, however, requires a means of testing it.
+Lean provides a built-in function called `dbgTraceIfShared` with the following signature:
+```output info
+{{#example_out Examples/ProgramsProofs/InsertionSort.lean dbgTraceIfSharedSig}}
+```
+It takes a string and a value as arguments, and prints a message that uses the string to standard error if the value has more than one reference, returning the value.
+This is not, strictly speaking, a pure function.
+However, it is intended to be used only during development to check that a function is in fact able to re-use memory rather than allocating.
+
+
+
+
